src/tree_of_strategy.lean
@@ -1,0 +1,154 @@
+import reducibility function  data.list.basic
+
+open encodable denumerable t_reducible
+
+local attribute [simp] set.set_of_app_iff
+
+@[derive decidable_eq]
+inductive infinity : Type
+| infinity : infinity
+
+@[derive decidable_eq]
+inductive zero : Type
+| zero : zero
+
+def Tree' : ℕ → Type
+| 0       := zero
+| (n + 1) := list (Tree' n ⊕ infinity)
+
+instance : ∀ n, decidable_eq (Tree' n)
+| 0       := zero.decidable_eq
+| (n + 1) := @list.decidable_eq _ (@sum.decidable_eq _ (Tree'.decidable_eq n) infinity _)
+
+def Tree (n : ℕ) := Tree' (n + 1)
+
+def subTree {n} (η : Tree n) := { μ : Tree n // μ <:+ η }
+
+instance : has_zero (zero ⊕ infinity) := ⟨sum.inl zero.zero⟩
+instance {n} : has_emptyc (Tree n) := ⟨[]⟩
+
+notation `∞` := sum.inr infinity.infinity
+
+
+#check @list.rec_on
+
+
+
+@[elab_as_eliminator]
+theorem Tree'.rec_on {n} {motive : Tree' (n+1) → Sort*} (μ : Tree' (n + 1))
+  (nil : motive [])
+  (cons₁ : Π (ν : Tree' n) (μ : Tree' (n + 1)), motive μ → motive (sum.inl ν :: μ))
+  (cons₂ : Π (μ : Tree' (n + 1)), motive μ → motive (∞ :: μ)) : motive μ :=
+begin
+  induction μ with ν μ IH, refine nil,
+  cases ν, { refine cons₁ ν μ IH },
+  { cases ν, refine cons₂ μ IH }
+end
+
+@[elab_as_eliminator]
+theorem Tree.rec_on {n} {motive : Tree (n+1) → Sort*} (μ : Tree (n + 1))
+  (nil : motive [])
+  (cons₁ : Π (ν : Tree n) (μ : Tree (n + 1)), motive μ → motive (sum.inl ν :: μ))
+  (cons₂ : Π (μ : Tree (n + 1)), motive μ → motive (∞ :: μ)) : motive μ :=
+@Tree'.rec_on (n + 1) motive μ nil cons₁ cons₂
+
+@[elab_as_eliminator]
+theorem Tree'.rec_on₁ {motive : Tree 1 → Sort*} (μ : Tree 1) 
+  (nil : motive (∅ : Tree 1))
+  (cons₁ : Π (ν : Tree 0) (μ : Tree 1), motive μ → motive (sum.inl ν :: μ))
+  (cons₂ : Π (μ : Tree 1), motive μ → motive (∞ :: μ : Tree 1)) : motive μ :=
+@Tree'.rec_on 1 motive μ nil cons₁ cons₂
+
+@[simp] def list.foldl' {α : Type*} (f : α → α → α) : list α → option α
+| []        := none
+| (a :: as) := if h : (list.foldl' as).is_some then f (option.get h) a else a
+
+structure strategy (R : Type*) :=
+(par₀ : Tree 0 → ℕ)
+(par₁ : Tree 1 → ℕ)
+(requirement : Tree 1 × ℕ → R)
+(computation : Tree 0 × R → Tree 0 × R → Prop)
+(inf : Tree 1 × ℕ → Tree 1 × ℕ → Tree 1 × ℕ)
+
+namespace strategy
+variables {R : Type*} (S : strategy R)
+
+@[reducible] def out {n} (μ η: Tree n) (ν : Tree' n ⊕ infinity) : Prop := ν :: μ <:+ η
+notation `out[` η `] ` μ ` ↝ ` ν := out μ η ν
+
+namespace approx
+variables υ : Π (n : ℕ) (η : Tree 0) (h : η.length < n), option (Tree 1)
+
+def weight (μ : Tree 1) : Π (η : Tree 0) (υ : subTree η → option (Tree 1)), ℕ
+| []       _ := 0
+| (_ :: η) υ := weight η (λ ν, υ ⟨ν.val, list.suffix_cons_iff.mpr(or.inr ν.property)⟩) +
+  (if υ ⟨η, by simp⟩ = ↑μ then 1 else 0)
+
+/--
+def weight (η : Tree 1) : Tree 0 → ℕ
+| []       := 0
+| (_ :: μ) := weight μ + (if υ μ = ↑η then 1 else 0)
+-/
+
+def is_exists_inv_infinity (η : Tree 1) : Tree 0 → option (Tree 0)
+| []               := none
+| (sum.inl _ :: μ) := is_exists_inv_infinity μ
+| (∞ :: μ)        :=
+    if (is_exists_inv_infinity μ).is_some then is_exists_inv_infinity μ
+    else if υ μ = ↑η then some μ else none
+
+lemma is_exists_inv_infinity_infinity (η : Tree 1) (μ : Tree 0) {μ₀ : Tree 0}
+  (h1 : out[μ] μ₀ ↝ ∞) (h2 : υ μ₀ = η) : (is_exists_inv_infinity υ η μ).is_some :=
+begin
+  induction μ with ν μ IH μ IH generalizing μ₀,
+  { exfalso, simp[out] at*, exact h1 },
+  cases ν,
+  { simp[is_exists_inv_infinity],
+    have : ∞ :: μ₀ = sum.inl ν :: μ ∨ out[μ] μ₀ ↝ ∞, from list.suffix_cons_iff.mp h1,
+    cases this,
+    { simp at*, exfalso, exact this },
+    { refine IH this h2 } },
+  { cases ν, simp[is_exists_inv_infinity] at*,
+    cases C : (is_exists_inv_infinity υ η μ).is_some; simp[C],
+    { have : ∞ :: μ₀ = ∞ :: μ ∨ out[μ] μ₀ ↝ ∞, from list.suffix_cons_iff.mp h1,
+      cases this,
+      { simp at*, rcases this with rfl, simp[h2] },
+      { exfalso, have := IH this h2, exact bool_iff_false.mpr C this } } }
+end
+
+def lambda' (η : Tree 0) : ℕ → Tree 1
+| 0       := []
+| (n + 1) :=
+    if 0 < weight υ (lambda' n) η then
+      if h : (is_exists_inv_infinity υ (lambda' n) η).is_some then
+        sum.inl (option.get h) :: lambda' n
+      else ∞ :: lambda' n
+    else lambda' n 
+
+def lambda (η : Tree 0) : Tree 1 := lambda' υ η η.length
+
+def assign (η : Tree 0) : Tree 1 → option (Tree 1 × ℕ)
+| []               := none
+| (sum.inl _ :: μ) := assign μ
+| (∞ :: μ)        :=
+  if h : (assign μ).is_some then S.inf (option.get h) (μ, weight υ μ η) else
+  some (μ, weight υ μ η)
+
+def assign_eq (η : Tree 0) : Tree 1 → option (Tree 1 × ℕ) := λ μ,
+if h : (assign S υ η μ).is_some then S.inf (option.get h) (μ, weight υ μ η) else
+  some (μ, weight υ μ η)
+
+def up (η : Tree 0) : option (Tree 1 × ℕ) := assign_eq S υ η (lambda υ η)
+
+def requirement (η : Tree 0) : option R := (up S υ η).map S.requirement
+
+end approx
+
+def up : Tree 0 → option (Tree 1 × ℕ)
+| [] 
+
+
+
+end strategy
+
+
